Fix spill sim

theories/Spilling/SpillSim.v
@@ -3,367 +3,135 @@ Require Import IL Annotation LabelsDefined.
 Require Import Liveness.Liveness TrueLiveness SimI.
 Require Import RenamedApart.
 Require Import SetUtil SpillSound ReconstrLive DoSpill ReconstrLiveUtil.
+Require Export SpillMovesAgree.
 
 Set Implicit Arguments.
 Unset Printing Records.
 
+Fixpoint extend_list X (L:list X) (Z:params) (RM : ⦃var⦄ * ⦃var⦄)
+  : list X
+  :=
+    match L, Z with
+    | l::L, z::Z => if [z ∈ fst RM ∩ snd RM]
+             then l::l::extend_list L Z RM
+             else l::extend_list L Z RM
+    | _, _ => nil
+    end.
+
 (** * SpillSim *)
 
-Lemma agree_on_eq_oval (D:set var) (f g: var -> option val)
-  : agree_on _eq D f g
-    -> agree_on eq D f g.
+Lemma extend_list_length X (L:list X) (RM : ⦃nat⦄ * ⦃nat⦄) (Z : params)
+      (NoDup:NoDupA eq Z) (Len:❬L❭ = ❬Z❭)
+  : ❬extend_list L Z RM❭ = ❬Z❭ + cardinal (of_list Z ∩ (fst RM ∩ snd RM)).
 Proof.
-  intros; hnf; intros.
-  eapply H in H0. inv H0; eauto; simpl in *; congruence.
-Qed.
-
-Lemma sim_write_moves D r L V s L' V' s' xl yl (Len:❬xl❭ = ❬yl❭)
-  : (forall (V'':onv val), agree_on eq D (V'[xl <-- lookup_list V' yl]) V''
-                        -> paco3 (sim_gen (S':=I.state)) r Sim (L, V, s) (L', V'', s'))
-    -> defined_on (of_list yl) V'
-    -> disj (of_list xl) (of_list yl)
-    -> NoDupA _eq xl
-    -> paco3 (sim_gen (S':=I.state)) r Sim (L, V, s)
-            (L', V', write_moves xl yl s').
-Proof.
-  intros SIM Def Disj Uniq.
-  length_equify. general induction Len.
-  - simpl in *. eapply SIM; eauto.
-  - simpl in *; dcr; invt NoDupA.
-    edestruct Def; [cset_tac|].
-    pone_step_right; simpl. rewrite <- H.
-    eapply IHLen; intros; eauto using injective_on_incl.
-    eapply SIM.
-    + rewrite <- update_nodup_commute_eq; simpl; eauto with len.
-      erewrite lookup_list_agree; eauto.
-      symmetry. eapply agree_on_update_dead; eauto.
-      eapply disj_not_in.
-      eapply disj_incl; eauto with cset.
-    + rewrite H; eapply defined_on_update_some;
-        eauto using defined_on_incl with cset.
-    + eapply disj_incl; eauto with cset.
-Qed.
-
-Lemma sim_I_moves (slot : var -> var) k Λ ZL r L L' V V' R M s sl ib
-  : spill_sound k ZL Λ (R,M) s sl
-    -> injective_on (getSp sl ∪ getL sl) slot
-    -> disj (getSp sl ∪ getL sl) (map slot (getSp sl ∪ getL sl))
-    -> defined_on (getSp sl ∪ (map slot (getL sl) \ map slot (getSp sl))) V'
-    -> (forall V'', agree_on eq (R ∪ map slot M ∪ map slot (getSp sl) ∪ getL sl)
-                       (V' [slot ⊝ elements (getSp sl) <-- lookup_list V' (elements (getSp sl))]
-                           [elements (getL sl) <-- lookup_list (V'[slot ⊝ elements (getSp sl) <-- lookup_list V' (elements (getSp sl))]) (slot ⊝ elements (getL sl))]) V''
-              -> paco3 (sim_gen (S':=I.state)) r Sim (L, V, s)
-                      (L', V'', do_spill slot s (setTopAnn sl ({}, {}, snd (getAnn sl))) ib))
-    -> sim r Sim (L, V, s) (L', V', do_spill slot s sl ib).
-Proof.
-  simpl. unfold reconstr_live_do_spill. unfold sim. revert_except s.
-  intros ? ? ? ? ? ? ? ? ? ? ? ? ? SPS Inj Disj Def SIM.
-  rewrite do_spill_extract_writes.
-  exploit L_sub_SpM; eauto.
-  exploit Sp_sub_R; eauto.
-  eapply (@sim_write_moves (R ∪ map slot M ∪ map slot (getSp sl) ∪ map slot (getL sl)));
-    try rewrite ?of_list_map, of_list_elements; eauto. eauto with len.
-  intros ? Agr3.
-  eapply (@sim_write_moves (R ∪ map slot M ∪ map slot (getSp sl) ∪ getL sl)); try rewrite ?of_list_map, of_list_elements; eauto. eauto with len.
-  intros ? Agr4.
-  - rewrite update_with_list_agree in Agr4; eauto;
-      [| symmetry; eapply agree_on_incl; eauto; clear; rewrite of_list_elements; cset_tac
-       |eauto with len].
-    erewrite <- (lookup_list_agree) in Agr4.
-    eapply SIM; eauto.
-    rewrite of_list_map, of_list_elements; eauto.
-    eapply agree_on_incl; eauto with cset.
-  - eapply defined_on_agree_eq; eauto using agree_on_incl with cset.
-    rewrite (incl_union_minus _ _ (map slot (getSp sl))).
-    eapply defined_on_union.
-    + hnf; intros.
-      rewrite <- (of_list_elements _ (getSp sl)) in H1.
-      rewrite <- of_list_map in H1; eauto.
-      edestruct update_with_list_lookup_in_list; try eapply H1; dcr.
-      Focus 2. rewrite H5. inv_get. eapply get_elements_in in H3.
-      rewrite lookup_list_map in H4; inv_get.
-      eapply get_elements_in in H4.
-      eauto with cset.
-      eauto with len.
-    + hnf; intros.
-      rewrite lookup_set_update_not_in_Z; eauto.
-      eapply Def; eauto with cset.
-      rewrite of_list_map, of_list_elements; eauto.
-      revert H1; clear_all; cset_tac.
-  - eapply disj_incl; eauto with cset.
-  - eapply elements_3w.
-  - eauto using defined_on_incl with cset.
-  - symmetry.
-     eapply disj_incl; eauto with cset.
-  - eapply injective_nodup_map; eauto.
-    rewrite of_list_elements. eauto using injective_on_incl with cset.
-    eapply elements_3w.
-Qed.
-
-Instance proper_onv (ϱ:var -> option val)
-  : (@Proper (forall _ : var, option val)
-             (@respectful var (option val) (@_eq var (@SOT_as_OT var (@eq nat) nat_OrderedType))
-                          (@eq (option val))) ϱ) | 0.
-Proof.
-  intuition.
-Qed.
-
-Instance proper_onv' (ϱ:var -> option val)
-  : @Proper (forall _ : var, option val)
-            (@respectful var (option val) (@_eq var (@SOT_as_OT var (@eq nat) nat_OrderedType))
-                         (@_eq (option val) (@option_OrderedType val OrderedType_int))) ϱ | 0.
-Proof.
-  intuition.
-Qed.
-
-Lemma load_agree_after_spill_load (slot : var -> var) (V V':var->option val) VD R M Sp L0
-      (Inj : injective_on VD slot)
-      (Agr1 : agree_on eq R V V')
-      (Agr2 : agree_on eq M V (fun x : var => V' (slot x)))
-      (VDincl:Sp ∪ L0 [<=] VD) (SpR:Sp [<=] R) (LSpM:L0 [<=] Sp ∪ M)
-  : agree_on eq L0 V
-             (V' [slot ⊝ elements Sp <-- V' ⊝ elements Sp]
-                 [elements L0 <-- V' [slot ⊝ elements Sp <-- V' ⊝ elements Sp]
-                           ⊝ slot ⊝ elements L0]).
-Proof.
-  eapply agree_on_update_list; try eapply proper_onv; eauto with len.
-  rewrite of_list_elements. eapply agree_on_empty; eauto with cset.
-  rewrite !lookup_list_map. rewrite map_map. rewrite <- !lookup_list_map.
-  eapply lookup_list_agree. rewrite lookup_list_map.
-  rewrite of_list_elements.
-  etransitivity; [| eapply agree_on_eq_oval, agree_on_update_list_map];
-    [ | eauto with len | eapply proper_var | eapply proper_onv'
-      | eapply injective_on_incl; eauto; rewrite <- VDincl, of_list_elements; clear; cset_tac ].
-  rewrite (set_decomp Sp).
-  eapply agree_on_union.
-  ++ rewrite lookup_list_map.
-    etransitivity; [eapply agree_on_incl; [ eapply Agr1| rewrite <- SpR; clear; cset_tac]|].
-    eapply agree_on_update_list; [ eapply proper_onv | eauto with len |
-                                   | rewrite lookup_list_map; reflexivity ].
-    rewrite of_list_elements. eapply agree_on_empty; clear; cset_tac.
-  ++ rewrite lookup_list_map.
-    eapply agree_on_update_list_dead.
-    eapply agree_on_incl; eauto. rewrite LSpM. clear; cset_tac.
-    rewrite of_list_elements. hnf; intros; cset_tac.
-Qed.
-
-Lemma regs_untouched_after_spill_load (slot : var -> var) (V V' V'':var->option val) VD R M K Sp L0
-      (Agr3 : agree_on eq (R ∪ map slot M ∪ map slot Sp ∪ L0)
-                       (V' [slot ⊝ elements Sp <-- V' ⊝ elements Sp]
-                           [elements L0 <-- V' [slot ⊝ elements Sp <-- V' ⊝ elements Sp]
-                                     ⊝ slot ⊝ elements L0]) V'')
-      (Disj : disj VD (map slot VD)) (Incl : R ∪ M [<=] VD)
-      (Agr1 : agree_on eq R V V')
-      (VDincl:Sp ∪ L0 [<=] VD)
-  :  agree_on eq ((R \ K) \ L0) V V''.
-Proof.
-  etransitivity; [eapply agree_on_incl; [eapply Agr1| clear; cset_tac]|].
-  etransitivity; [|eapply agree_on_incl; [eapply Agr3| clear; cset_tac]].
-  eapply agree_on_update_list_dead.
-  eapply agree_on_update_list_dead. reflexivity.
-  rewrite of_list_map, of_list_elements; eauto.
-  symmetry. eapply disj_incl; eauto; only 2: eauto with cset.
-  rewrite <- Incl. clear; cset_tac.
-  rewrite of_list_elements. clear; hnf; intros; cset_tac.
-Qed.
-
-Lemma regs_agree_after_spill_load (slot : var -> var) (V V' V'':var -> option val) VD R M K Sp L0
-      (Agr3 : agree_on eq (R ∪ map slot M ∪ map slot Sp ∪ L0)
-                       (V' [slot ⊝ elements Sp <-- V' ⊝ elements Sp]
-                           [elements L0 <-- V' [slot ⊝ elements Sp <-- V' ⊝ elements Sp]
-                                     ⊝ slot ⊝ elements L0]) V'')
-      (Inj : injective_on VD slot) (Disj : disj VD (map slot VD)) (Incl : R ∪ M [<=] VD)
-      (Agr1 : agree_on eq R V V')
-      (Agr2 : agree_on eq M V (fun x : var => V' (slot x)))
-      (VDincl:Sp ∪ L0 [<=] VD) (SpR:Sp [<=] R) (LSpM:L0 [<=] Sp ∪ M)
-  : agree_on eq (R \ K ∪ L0) V V''.
-Proof.
-  etransitivity; [|eapply agree_on_incl; [eapply Agr3| clear; cset_tac]].
-  rewrite union_comm, union_exclusive.
-  eapply agree_on_union.
-  -- eapply load_agree_after_spill_load; eauto.
-  -- eapply regs_untouched_after_spill_load; eauto.
-     reflexivity.
-Qed.
-
-Lemma spills_agree_after_spill_load (slot : var -> var) (V V' V'':var->option val) VD R M Sp L0
-      (Inj : injective_on VD slot) (Disj : disj VD (map slot VD)) (Incl : R ∪ M [<=] VD)
-      (Agr1 : agree_on eq R V V')
-      (Agr2 : agree_on eq M V (fun x : var => V' (slot x)))
-      (VDincl:Sp ∪ L0 [<=] VD) (SpR:Sp [<=] R) (LSpM:L0 [<=] Sp ∪ M)
-      (Agr3 : agree_on eq (R ∪ map slot M ∪ map slot Sp ∪ L0)
-                       (V' [slot ⊝ elements Sp <-- V' ⊝ elements Sp]
-                           [elements L0 <-- V' [slot ⊝ elements Sp <-- V' ⊝ elements Sp]
-                                     ⊝ slot ⊝ elements L0]) V'')
-  : agree_on eq Sp V (fun x : var => V'' (slot x)).
-Proof.
-  eapply agree_on_comp; eauto; [ symmetry; eapply agree_on_incl; eauto; clear_all; cset_tac | ].
-  etransitivity; [eapply agree_on_incl; [eapply Agr1| eauto with cset]|].
-  eapply agree_on_update_list_dead_slot; eauto.
-  etransitivity; [| eapply agree_on_eq_oval, agree_on_update_list_map];
-    [ | eauto with len | eapply proper_var | eapply proper_onv'
-      | eapply injective_on_incl; eauto; rewrite <- VDincl, of_list_elements;
-        clear; cset_tac ].
-  eapply agree_on_update_list; [ eapply proper_onv | eauto with len |
-                                 | rewrite lookup_list_map; reflexivity ].
-  eapply agree_on_empty. rewrite of_list_elements. cset_tac.
-  eapply disj_incl; eauto with cset.
-  rewrite of_list_elements, <- Incl, LSpM, <- SpR; reflexivity.
-Qed.
-
-Lemma mem_untouched_after_spill_load (slot : var -> var) (V V' V'':var->option val) VD R M Sp L0
-      (Inj : injective_on VD slot) (Disj : disj VD (map slot VD)) (Incl : R ∪ M [<=] VD)
-      (Agr1 : agree_on eq R V V')
-      (Agr2 : agree_on eq M V (fun x : var => V' (slot x)))
-      (VDincl:Sp ∪ L0 [<=] VD) (SpR:Sp [<=] R) (LSpM:L0 [<=] Sp ∪ M)
-      (Agr3 : agree_on eq (R ∪ map slot M ∪ map slot Sp ∪ L0)
-                       (V' [slot ⊝ elements Sp <-- V' ⊝ elements Sp]
-                           [elements L0 <-- V' [slot ⊝ elements Sp <-- V' ⊝ elements Sp]
-                                     ⊝ slot ⊝ elements L0]) V'')
-  : agree_on eq (M \ Sp) V (fun x : var => V'' (slot x)).
-Proof.
-  etransitivity; [eapply agree_on_incl; [eapply Agr2| eauto with cset ]|].
-  eapply agree_on_comp_both; eauto using proper_onv.
-  etransitivity; [| eapply agree_on_incl; [eapply Agr3| eauto]].
-  - eapply agree_on_update_list_dead.
-    eapply agree_on_update_list_dead. reflexivity.
-    rewrite of_list_map, of_list_elements; eauto.
-    intros.
-    eapply injective_disj; eauto.
-    hnf; intros; cset_tac.
-    eapply injective_on_incl; eauto. rewrite <- Incl. rewrite SpR at 1.
-    cset_tac.
-    rewrite of_list_elements.
-    eapply disj_incl; eauto.
-    rewrite <- Incl, LSpM, <- SpR. eauto. eauto with cset.
-  - rewrite minus_incl. clear. cset_tac.
-Qed.
-
-Lemma mem_agrees_after_spill_load (slot : var -> var) (V V' V'':var->option val) VD R M Sp L0
-      (Agr3 : agree_on eq (R ∪ map slot M ∪ map slot Sp ∪ L0)
-                       (V' [slot ⊝ elements Sp <-- V' ⊝ elements Sp]
-                           [elements L0 <-- V' [slot ⊝ elements Sp <-- V' ⊝ elements Sp]
-                                     ⊝ slot ⊝ elements L0]) V'')
-      (Inj : injective_on VD slot) (Disj : disj VD (map slot VD)) (Incl : R ∪ M [<=] VD)
-      (Agr1 : agree_on eq R V V')
-      (Agr2 : agree_on eq M V (fun x : var => V' (slot x)))
-      (VDincl:Sp ∪ L0 [<=] VD) (SpR:Sp [<=] R) (LSpM:L0 [<=] Sp ∪ M)
-  : agree_on eq (Sp ∪ M) V (fun x : var => V'' (slot x)).
-Proof.
-  rewrite union_exclusive.
-  eapply agree_on_union.
-  -- eapply spills_agree_after_spill_load; try eapply Agr3; eauto.
-  -- eapply mem_untouched_after_spill_load; try eapply Agr3; eauto.
+  general induction Len; simpl; eauto.
+  inv NoDup.
+  repeat cases; simpl; rewrite IHLen; eauto.
+  - rewrite cap_special_in; eauto.
+    rewrite add_cardinal_2; eauto. cset_tac.
+  - rewrite cap_special_notin; eauto.
 Qed.
 
 
-Lemma mem_agrees_after_spill_load_update (slot : var -> var) (V V' V'':var->option val) VD R M Sp L0 x v
-      (Agr5 : agree_on eq (Sp ∪ M) V (fun x : var => V'' (slot x)))
-      (Disj : disj VD (map slot VD)) (Incl : R ∪ M [<=] VD) (NotIn: x ∉ Sp ∪ M)
-      (xIn:x ∈ VD)
-      (Agr1 : agree_on eq R V V')
-      (Agr2 : agree_on eq M V (fun x : var => V' (slot x)))
-      (VDincl:Sp ∪ L0 [<=] VD) (SpR:Sp [<=] R) (LSpM:L0 [<=] Sp ∪ M)
-      (Agr3 : agree_on eq (R ∪ map slot M ∪ map slot Sp ∪ L0)
-                       (V' [slot ⊝ elements Sp <-- V' ⊝ elements Sp]
-                           [elements L0 <-- V' [slot ⊝ elements Sp <-- V' ⊝ elements Sp]
-                                     ⊝ slot ⊝ elements L0]) V'')
-  : agree_on eq (Sp ∪ M) (V [x <- ⎣ v ⎦]) (fun x0 : var => (V'' [x <- ⎣ v ⎦]) (slot x0)).
+Lemma slot_lift_params_extend_list_length X slot RM Z (L:list X)
+      (Len:❬Z❭ = ❬L❭)
+  : ❬slot_lift_params slot RM Z❭ = ❬extend_list L Z RM❭.
 Proof.
-  eapply agree_on_update_dead_both_comp_right; eauto.
-  eapply disj_incl; eauto. rewrite SpR, Incl. revert xIn; clear. cset_tac.
-  rewrite SpR, Incl. cset_tac.
+  general induction Len; simpl; eauto.
+  repeat cases; eauto; simpl; eauto.
 Qed.
 
-Lemma RKL_incl X `{OrderedType X} (R K L D D':set X)
-  :  R \ K ∪ L ⊆ R ∪ D ∪ D' ∪ L.
-Proof.
-  cset_tac.
-Qed.
-
-Hint Resolve RKL_incl | 0: cset.
-
-Lemma defined_on_after_spill_load (slot : var -> var) (V V' V'':var->option val) VD R M Sp L0  K
-      (Agr5 : agree_on eq (Sp ∪ M) V (fun x : var => V'' (slot x)))
-      (Disj : disj VD (map slot VD)) (Incl : R ∪ M [<=] VD)
-      (Agr1 : agree_on eq R V V') (Def : defined_on (R ∪ map slot M) V')
-      (Agr2 : agree_on eq M V (fun x : var => V' (slot x)))
-      (VDincl:Sp ∪ L0 [<=] VD) (SpR:Sp [<=] R) (LSpM:L0 [<=] Sp ∪ M)
-      (Agr3 : agree_on eq (R ∪ map slot M ∪ map slot Sp ∪ L0)
-                       (V' [slot ⊝ elements Sp <-- V' ⊝ elements Sp]
-                           [elements L0 <-- V' [slot ⊝ elements Sp <-- V' ⊝ elements Sp]
-                                     ⊝ slot ⊝ elements L0]) V'')
-  : defined_on (R \ K ∪ L0 ∪ map slot (Sp ∪ M)) V''.
-Proof.
-  assert (defined_on Sp V') as DefSp by eauto using defined_on_incl with cset.
-  rewrite union_exclusive.
-  eapply defined_on_union.
-  -- eapply defined_on_agree_eq; [|eapply agree_on_incl;[eapply Agr3|eauto with cset]].
-     rewrite union_comm, union_exclusive. eapply defined_on_union.
-     ++ eapply defined_on_update_list'; eauto with len.
-       rewrite of_list_elements. clear; hnf; intros; cset_tac.
-       eapply defined_on_defined. clear; intuition.
-       rewrite of_list_map, of_list_elements; eauto.
-       eapply defined_on_update_list'; eauto with len.
-       rewrite of_list_map, of_list_elements; eauto.
-       rewrite LSpM. eapply (defined_on_incl Def); eauto.
-       rewrite map_union; eauto. clear; cset_tac.
-       eapply defined_on_defined. clear; intuition. eauto.
-       rewrite of_list_elements. eauto.
-     ++ eapply defined_on_agree_eq; [| eapply agree_on_update_list_dead; try reflexivity].
-       eapply defined_on_update_list'; eauto with len.
-       rewrite of_list_map, of_list_elements; eauto.
-       eapply (defined_on_incl Def). clear; cset_tac.
-       eapply defined_on_defined. clear; intuition. eauto.
-       rewrite of_list_elements. eauto.
-       rewrite of_list_elements. eauto. clear; hnf; intros; cset_tac.
-  -- rewrite map_union; eauto.
-     eapply defined_on_agree_eq; [ | eapply agree_on_incl; [ eapply Agr3| clear; cset_tac]];
-       eauto.
-     eapply defined_on_agree_eq; [| eapply agree_on_update_list_dead; try reflexivity].
-     eapply defined_on_update_list'; eauto with len.
-     rewrite of_list_map, of_list_elements; eauto.
-     eapply (defined_on_incl Def). clear; cset_tac.
-     eapply defined_on_defined. clear; intuition. eauto.
-     rewrite of_list_elements. eauto.
-     rewrite of_list_elements. clear; hnf; intros; cset_tac.
-Qed.
-
-Lemma omap_slotlift (slot : var -> var) (V V'':onv val) xl Yv ib (Len:❬xl❭=❬ib❭) Sl R K L0 Sp M
-      (Agr4 : agree_on eq (R \ K ∪ L0) V V'')
-      (Agr5 : agree_on eq (Sp ∪ M) V (fun x : var => V'' (slot x)))
-      (FVincl: of_list xl [<=] Sl ∪ (R \ K ∪ L0))
-      (Slincl:Sl [<=] Sp ∪ M)
+Lemma omap_slotlift (slot : var -> var) (V V'':onv val) Yv (xl Z:params) (Len:❬xl❭=❬Z❭) RM RMapp
+      (Agr4 : agree_on eq (fst RMapp) V V'')
+      (Agr5 : agree_on eq (snd RMapp) V (fun x : var => V'' (slot x)))
+      (FVincl: of_list xl [<=] fst RMapp ∪ snd RMapp)
   : omap (op_eval V) (Var ⊝ xl) = Some Yv
-    -> omap (op_eval V'') (slot_lift_args slot Sl ⊝ extend_args (Var ⊝ xl) ib)
-      = Some (extend_args Yv ib).
+    -> omap (op_eval V'') (slot_lift_args slot RM RMapp (Var ⊝ xl) Z)
+      = Some (extend_list Yv Z RM).
 Proof.
   intros.
-  length_equify.
   general induction Len; simpl in *; eauto;
-    monad_inv H; simpl in *.
-  repeat (cases; simpl).
-  - rewrite <- Agr5; [ rewrite EQ | rewrite <- Slincl; eauto]; simpl.
-    erewrite IHLen; eauto; [ | rewrite <- FVincl; eauto with cset ]; eauto.
-  - rewrite <- Agr4; [ rewrite EQ | ]; simpl.
-    erewrite IHLen; eauto; [ | rewrite <- FVincl; eauto with cset ]; eauto.
-    assert (x ∈ Sl ∪ (R \ K ∪ L0)) by (rewrite <- FVincl; cset_tac).
-    revert NOTCOND H. clear; cset_tac.
-  - rewrite <- Agr5; [ rewrite EQ | rewrite <- Slincl; eauto]; simpl.
-    erewrite IHLen; eauto; [ | rewrite <- FVincl; eauto with cset ]; eauto.
-  - rewrite <- Agr4; [ rewrite EQ | ]; simpl.
-    erewrite IHLen; eauto; [ | rewrite <- FVincl; eauto with cset ]; eauto.
-    assert (x ∈ Sl ∪ (R \ K ∪ L0)) by (rewrite <- FVincl; cset_tac).
-    revert NOTCOND H. clear; cset_tac.
+    monad_inv H; simpl in *. unfold choose_y.
+  cases; simpl.
+  - assert (y ∈ fst RM /\ y ∈ snd RM) by (revert COND; clear_all; cset_tac).
+    destruct H. repeat (cases; simpl).
+    + rewrite <- Agr4; eauto. rewrite EQ. simpl.
+      erewrite IHLen; eauto; [ | rewrite <- FVincl; eauto with cset ]; eauto.
+    + rewrite <- Agr5; eauto.
+      * rewrite EQ; eauto; simpl.
+        erewrite IHLen; eauto; [ | rewrite <- FVincl; eauto with cset ]; eauto.
+      * revert FVincl NOTCOND. clear_all. cset_tac.
+  - assert ((y ∈ fst RM -> y ∈ snd RM -> False))
+      by (revert NOTCOND; clear_all; cset_tac).
+    unfold choose_y; repeat cases; simpl; eauto.
+    + rewrite <- Agr4; [ rewrite EQ | ]; simpl; eauto.
+      erewrite IHLen; eauto; [ | rewrite <- FVincl; eauto with cset ]; eauto.
+    + rewrite <- Agr5; [ rewrite EQ | eauto]; simpl.
+      erewrite IHLen; eauto; [ | rewrite <- FVincl; eauto with cset ]; eauto.
+      cset_tac.
+    + rewrite <- Agr4; [ rewrite EQ | ]; simpl; eauto.
+      erewrite IHLen; eauto; [ | rewrite <- FVincl; eauto with cset ]; eauto.
+    + rewrite <- Agr5; [ rewrite EQ | eauto]; simpl.
+      erewrite IHLen; eauto; [ | rewrite <- FVincl; eauto with cset ]; eauto.
+      cset_tac.
+    + rewrite <- Agr5; [ rewrite EQ | eauto]; simpl.
+      erewrite IHLen; eauto; [ | rewrite <- FVincl; eauto with cset ]; eauto.
+    + rewrite <- Agr4; [ rewrite EQ | ]; simpl; eauto.
+      erewrite IHLen; eauto; [ | rewrite <- FVincl; eauto with cset ]; eauto.
+      cset_tac.
 Qed.
+
+
+
+
+Lemma update_with_list_lookup_in_list_first_slot (slot:var->var)
+      A (E:onv A) n (R M:set var)
+      Z (Y:list A) z
+: length Z = length Y
+  -> get Z n z
+  -> z ∈ R
+  -> disj (of_list Z) (map slot (of_list Z))
+  -> (forall n' z', n' < n -> get Z n' z' -> z' =/= z)
+  -> exists y, get Y n y
+         /\ E [slot_lift_params slot (R, M) Z <--
+                               Some ⊝ extend_list Y Z (R, M)] z = Some y.
+Proof.
+  intros Len Get In Disj First. length_equify.
+  general induction Len; simpl in *; isabsurd.
+  inv Get.
+  - exists y; repeat split; eauto using get.
+    cases; simpl.
+    + lud; eauto using get.
+    + cases; simpl.
+      * lud; eauto using get.
+  - edestruct (IHLen slot E n0) as [? [? ]]; eauto using get; dcr.
+    + eapply disj_incl; eauto with cset.
+    + intros. eapply (First (S n')); eauto using get. omega.
+    + exists x0. eexists; repeat split; eauto using get.
+      exploit (First 0); eauto using get; try omega.
+      cases; simpl.
+      * rewrite lookup_nequiv; eauto.
+        rewrite lookup_nequiv; eauto.
+        intro.
+        eapply (Disj z). eapply get_in_of_list in H3.
+        cset_tac. rewrite <- H2.
+        eapply map_iff; eauto. eexists x; split; eauto with cset.
+      * cases; simpl; lud.
+        -- rewrite lookup_nequiv; eauto.
+        -- exfalso.
+           eapply (Disj (slot x)). eapply get_in_of_list in H3.
+           rewrite <- H5. cset_tac.
+           eapply map_iff; eauto. eexists x; split; eauto with cset.
+        -- eauto.
+Qed.
+
 
 Lemma slot_lift_params_agree (slot : var -> var) X (E:onv X) E' R M Z VL (Len:❬Z❭=❬VL❭)
       (Agr2:agree_on eq (R \ of_list Z) E E')
       (Disj:disj (R ∪ of_list Z) (map slot (R ∪ of_list Z)))
       (Incl:of_list Z [<=] R ∪ M)
   : agree_on eq R (E [Z <-- Some ⊝ VL])
-             (E' [slot_lift_params slot (R, M) Z <--
-                  Some ⊝ extend_args VL (mark_elements Z (R ∩ M))]).
+             (E' [slot_lift_params slot (R, M) Z <-- Some ⊝ extend_list VL Z (R, M)]).
 Proof.
   hnf; intros.
   decide (x ∈ of_list Z).
@@ -396,7 +164,7 @@ Lemma update_with_list_lookup_in_list_first_slot' (slot : var -> var) A (E:onv A
   -> injective_on (of_list Z ∪ R ∪ M) slot
   -> (forall n' z', n' < n -> get Z n' z' -> z' =/= z)
   -> exists y, get Y n y /\ E [slot_lift_params slot (R, M) Z <--
-                  Some ⊝ extend_args Y (mark_elements Z (R ∩ M))] (slot z) = Some y.
+                  Some ⊝ extend_list Y Z (R, M)] (slot z) = Some y.
 Proof.
   intros Len Get In Disj Inj First. length_equify.
   general induction Len; simpl in *; isabsurd.
@@ -428,6 +196,8 @@ Proof.
         -- exfalso. eapply H2. eapply Inj; eauto with cset.
 Qed.
 
+
+
 Lemma slot_lift_params_agree_slot (slot : var -> var) X (E:onv X) E' R M Z VL (Len:❬Z❭=❬VL❭)
       (Agr2:agree_on eq (M \ of_list Z) E (fun x => E' (slot x)))
       (Disj:disj (of_list Z ∪ R ∪ M) (map slot (of_list Z ∪ R ∪ M)))
@@ -435,7 +205,7 @@ Lemma slot_lift_params_agree_slot (slot : var -> var) X (E:onv X) E' R M Z VL (L
       (Incl:of_list Z [<=] R ∪ M)
         : agree_on eq M (E [Z <-- Some ⊝ VL])
              (fun x => E' [slot_lift_params slot (R, M) Z <--
-                        Some ⊝ extend_args VL (mark_elements Z (R ∩ M))] (slot x)).
+                        Some ⊝ extend_list VL Z (R, M)] (slot x)).
 Proof.
   hnf; intros.
   decide (x ∈ of_list Z).
@@ -458,11 +228,12 @@ Proof.
       cset_tac.
 Qed.
 
+
 Instance SR (slot : var -> var) (VD:set var)
   : PointwiseProofRelationI (((set var) * (set var)) * params) := {
    ParamRelIP RMZ Z Z' := Z' = slot_lift_params slot (fst RMZ) Z /\ Z = snd RMZ;
    ArgRelIP V V' RMZ VL VL' :=
-     VL' = extend_args VL (mark_elements (snd RMZ) (fst (fst RMZ) ∩ snd (fst RMZ))) /\
+     VL' = extend_list VL (snd RMZ) (fst RMZ) /\
      agree_on eq (fst (fst RMZ) \ of_list (snd RMZ)) V V' /\
      agree_on eq (snd (fst RMZ) \ of_list (snd RMZ)) V (fun x => V' (slot x)) /\
      ❬VL❭ = ❬snd RMZ❭ /\
@@ -487,7 +258,7 @@ Lemma sim_I (slot : var -> var) k Λ ZL LV VD r L L' V V' R M s lv sl ra
     -> renamedApart s ra
     -> app_expfree s
     -> ann_R Subset1 lv ra
-    -> sim r Sim (L, V, s) (L', V', do_spill slot s sl (compute_ib ⊜ ZL Λ)).
+    -> sim r Sim (L, V, s) (L', V', do_spill slot s sl ZL Λ).
 Proof.
   simpl. unfold reconstr_live_do_spill. unfold sim.
   move VD before k. move s before VD. revert_until s.
@@ -512,15 +283,16 @@ Proof.
   rewrite map_union; eauto. clear; cset_tac.
   rewrite !lookup_list_map. intros ? Agr3.
   time (destruct s; invt spill_sound; invt spill_live; invt live_sound;
-        invt renamedApart; invt app_expfree; try invtc (@ann_R _ _ Subset1));
-    exploit regs_agree_after_spill_load as Agr4; eauto;
-      exploit mem_agrees_after_spill_load as Agr5; eauto;
-        simpl in *; rewrite !elements_empty; simpl.
+        invt renamedApart; invt app_expfree; try invtc (@ann_R _ _ Subset1);
+    (exploit regs_agree_after_spill_load as Agr4); try eassumption;
+      exploit mem_agrees_after_spill_load as Agr5; try eassumption;
+        simpl in *; rewrite !elements_empty; simpl).
   - destruct e; simpl in *.
     + eapply (sim_let_op il_statetype_I); eauto.
       * symmetry; eapply op_eval_agree; eauto using agree_on_incl.
       * intros. left.
-        eapply IH; eauto.
+        eapply (IH s); try eassumption.
+        -- eauto.
         -- eapply agree_on_update_same; eauto.
            eapply agree_on_incl; eauto.
            clear; cset_tac.
@@ -536,9 +308,10 @@ Proof.
            rewrite LSpM, SpR, <- Incl'. clear; cset_tac.
         -- pe_rewrite. rewrite <- RAincl.
            rewrite H18. clear; cset_tac.
-    + eapply (sim_let_call il_statetype_I); eauto.
+    + eapply (sim_let_call il_statetype_I).
       * symmetry; eapply omap_op_eval_agree; eauto using agree_on_incl.
-      * intros. left. eapply IH; eauto.
+      * intros. left. eapply (IH s); try eassumption.
+        -- eauto.
         -- eapply agree_on_update_same; eauto.
            eapply agree_on_incl; eauto.
            clear; cset_tac.
@@ -555,44 +328,45 @@ Proof.
         -- pe_rewrite. rewrite <- RAincl.
            rewrite H18. clear; cset_tac.
   - simpl in *.
-    eapply (sim_cond il_statetype_I); eauto.
+    eapply (sim_cond il_statetype_I).
     + symmetry; eapply op_eval_agree; eauto using agree_on_incl.
-    + intros; left. eapply IH; eauto.
+    + intros; left. eapply IH; try eassumption.
+      * eauto.
       * eapply defined_on_after_spill_load; eauto.
       * pe_rewrite. rewrite LSpM, SpR, <- Incl'. clear; cset_tac.
       * pe_rewrite. rewrite <- RAincl, <- H9. clear; cset_tac.
-    + intros; left. eapply IH; eauto.
+    + intros; left. eapply IH; try eassumption.
+      * eauto.
       * eapply defined_on_after_spill_load; eauto.
       * pe_rewrite. rewrite LSpM, SpR, <- Incl'. clear; cset_tac.
       * pe_rewrite. rewrite <- RAincl, <- H9. clear; cset_tac.
   - eapply labenv_sim_app; eauto using zip_get.
     intros; simpl in *. dcr; subst; repeat get_functional.
     split; eauto; intros.
-    erewrite get_nth; eauto using zip_get. unfold compute_ib. simpl.
+    erewrite !get_nth; eauto using zip_get.
     edestruct op_eval_var; eauto; subst.
-    erewrite omap_slotlift; eauto.
+    erewrite omap_slotlift; only 6: eauto.
     eexists; split; eauto. split; eauto.
-    erewrite <- sla_extargs_slp_length; eauto. instantiate (1:=M').
-    simpl. eauto with len.
+    eapply slot_lift_params_extend_list_length; eauto.
     split; eauto.
     split; eauto using agree_on_incl.
     split; eauto using agree_on_incl.
     split; eauto.
     eapply defined_on_incl.
     eapply defined_on_after_spill_load; eauto. instantiate (1:=K).
-    rewrite H10, H11. reflexivity.
-    unfold mark_elements. len_simpl. rewrite <- H16. eauto with len.
-    rewrite union_comm.
-    rewrite <- H13. eapply of_list_freeVars_vars.
+    rewrite H8, H11. reflexivity.
+    unfold mark_elements. len_simpl. rewrite <- H17. eauto with len.
+    simpl. eapply agree_on_incl; eauto.
+    simpl. eapply agree_on_incl; eauto. simpl.
+    rewrite <- H12. eapply of_list_freeVars_vars.
   - pno_step. simpl.
     erewrite op_eval_agree; [reflexivity| |reflexivity]. symmetry.
     eapply agree_on_incl; eauto using regs_agree_after_spill_load; eauto.
-  - eapply sim_fun_ptw; try eapply LSim; eauto.
-    + intros. left. rewrite <- zip_app; [| eauto with len].
-      eapply (IH s); eauto using agree_on_incl.
+  - eapply sim_fun_ptw; try eapply LSim; try eassumption.
+    + intros. left.
+      eapply (IH s); eauto.
       * eapply defined_on_after_spill_load; eauto.
       * pe_rewrite. rewrite LSpM, SpR, <- Incl'. clear; cset_tac.
-      * rewrite !zip_app; eauto with len.
       * pe_rewrite. rewrite <- RAincl, <- H25. clear; cset_tac.
     + intros. hnf; intros; simpl in *; dcr. subst.
       inv_get.
@@ -602,9 +376,9 @@ Proof.
       exploit H14 as In'; try eassumption; simpl in *; destruct In' as [In1 In2].
       exploit H2 as RA'; try eassumption.
       exploit (get_PIR2 H7) as EQ; only 1-2: eauto.
-      exploit H21 as In3; eauto. destruct In3 as [In3 _].
+      exploit H21 as In3; try eassumption.
+      destruct In3 as [In3 _].
       unfold merge in EQ. simpl in *.
-      rewrite <- zip_app; [| eauto with len].
       eapply IH; eauto.
       * eapply slot_lift_params_agree; only 1-2: eauto.
         -- eapply disj_incl; eauto.
@@ -624,9 +398,7 @@ Proof.
       * eapply defined_on_update_list'.
         -- len_simpl.
            edestruct H8; eauto; dcr. simpl in *.
-           rewrite countTrue_mark_elements; eauto.
-           rewrite slot_lift_params_length; eauto.
-           unfold mark_elements. eauto with len.
+           eapply slot_lift_params_extend_list_length; eauto.
         -- rewrite of_list_slot_lift_params; eauto.
            eapply defined_on_incl; eauto.
            rewrite <- EQ in In3; revert In3; clear.
@@ -638,7 +410,6 @@ Proof.
       * edestruct H8; eauto; dcr.
         simpl in *. rewrite EQ.
         exploit H33; eauto. eapply ann_R_get in H4. eauto.
-      * rewrite !zip_app; eauto with len.
       * edestruct H8; eauto; dcr.
         rewrite H3. simpl. rewrite union_comm. rewrite <- union_assoc.
         eapply union_incl_split.
