theories/Spilling/SpillMovesAgree.v
@@ -1,0 +1,328 @@
+Require Import CSet Util Fresh Filter Take MoreList OUnion AllInRel MapDefined MapUpdate Position.
+Require Import IL Annotation LabelsDefined.
+Require Import Liveness.Liveness TrueLiveness SimI.
+Require Import RenamedApart.
+Require Import SetUtil SpillSound ReconstrLive DoSpill ReconstrLiveUtil.
+
+Set Implicit Arguments.
+Unset Printing Records.
+
+Lemma agree_on_eq_oval (D:set var) (f g: var -> option val)
+  : agree_on _eq D f g
+    -> agree_on eq D f g.
+Proof.
+  intros; hnf; intros.
+  eapply H in H0. inv H0; eauto; simpl in *; congruence.
+Qed.
+
+Lemma sim_write_moves D r L V s L' V' s' xl yl (Len:❬xl❭ = ❬yl❭)
+  : (forall (V'':onv val), agree_on eq D (V'[xl <-- lookup_list V' yl]) V''
+                        -> paco3 (sim_gen (S':=I.state)) r Sim (L, V, s) (L', V'', s'))
+    -> defined_on (of_list yl) V'
+    -> disj (of_list xl) (of_list yl)
+    -> NoDupA _eq xl
+    -> paco3 (sim_gen (S':=I.state)) r Sim (L, V, s)
+            (L', V', write_moves xl yl s').
+Proof.
+  intros SIM Def Disj Uniq.
+  length_equify. general induction Len.
+  - simpl in *. eapply SIM; eauto.
+  - simpl in *; dcr; invt NoDupA.
+    edestruct Def; [cset_tac|].
+    pone_step_right; simpl. rewrite <- H.
+    eapply IHLen; intros; eauto using injective_on_incl.
+    eapply SIM.
+    + rewrite <- update_nodup_commute_eq; simpl; eauto with len.
+      erewrite lookup_list_agree; eauto.
+      symmetry. eapply agree_on_update_dead; eauto.
+      eapply disj_not_in.
+      eapply disj_incl; eauto with cset.
+    + rewrite H; eapply defined_on_update_some;
+        eauto using defined_on_incl with cset.
+    + eapply disj_incl; eauto with cset.
+Qed.
+
+Lemma sim_I_moves (slot : var -> var) k Λ ZL r L L' V V' R M s sl RML
+  : spill_sound k ZL Λ (R,M) s sl
+    -> injective_on (getSp sl ∪ getL sl) slot
+    -> disj (getSp sl ∪ getL sl) (map slot (getSp sl ∪ getL sl))
+    -> defined_on (getSp sl ∪ (map slot (getL sl) \ map slot (getSp sl))) V'
+    -> (forall V'', agree_on eq (R ∪ map slot M ∪ map slot (getSp sl) ∪ getL sl)
+                       (V' [slot ⊝ elements (getSp sl) <-- lookup_list V' (elements (getSp sl))]
+                           [elements (getL sl) <-- lookup_list (V'[slot ⊝ elements (getSp sl) <-- lookup_list V' (elements (getSp sl))]) (slot ⊝ elements (getL sl))]) V''
+              -> paco3 (sim_gen (S':=I.state)) r Sim (L, V, s)
+                      (L', V'', do_spill slot s (setTopAnn sl ({}, {}, snd (getAnn sl))) ZL RML))
+    -> sim r Sim (L, V, s) (L', V', do_spill slot s sl ZL RML).
+Proof.
+  simpl. unfold reconstr_live_do_spill. unfold sim. revert_except s.
+  intros ? ? ? ? ? ? ? ? ? ? ? ? ? SPS Inj Disj Def SIM.
+  rewrite do_spill_extract_writes.
+  exploit L_sub_SpM; eauto.
+  exploit Sp_sub_R; eauto.
+  eapply (@sim_write_moves (R ∪ map slot M ∪ map slot (getSp sl) ∪ map slot (getL sl)));
+    try rewrite ?of_list_map, of_list_elements; eauto. eauto with len.
+  intros ? Agr3.
+  eapply (@sim_write_moves (R ∪ map slot M ∪ map slot (getSp sl) ∪ getL sl)); try rewrite ?of_list_map, of_list_elements; eauto. eauto with len.
+  intros ? Agr4.
+  - rewrite update_with_list_agree in Agr4; eauto;
+      [| symmetry; eapply agree_on_incl; eauto; clear; rewrite of_list_elements; cset_tac
+       |eauto with len].
+    erewrite <- (lookup_list_agree) in Agr4.
+    eapply SIM; eauto.
+    rewrite of_list_map, of_list_elements; eauto.
+    eapply agree_on_incl; eauto with cset.
+  - eapply defined_on_agree_eq; eauto using agree_on_incl with cset.
+    rewrite (incl_union_minus _ _ (map slot (getSp sl))).
+    eapply defined_on_union.
+    + hnf; intros.
+      rewrite <- (of_list_elements _ (getSp sl)) in H1.
+      rewrite <- of_list_map in H1; eauto.
+      edestruct update_with_list_lookup_in_list; try eapply H1; dcr.
+      Focus 2. rewrite H5. inv_get. eapply get_elements_in in H3.
+      rewrite lookup_list_map in H4; inv_get.
+      eapply get_elements_in in H4.
+      eauto with cset.
+      eauto with len.
+    + hnf; intros.
+      rewrite lookup_set_update_not_in_Z; eauto.
+      eapply Def; eauto with cset.
+      rewrite of_list_map, of_list_elements; eauto.
+      revert H1; clear_all; cset_tac.
+  - eapply disj_incl; eauto with cset.
+  - eapply elements_3w.
+  - eauto using defined_on_incl with cset.
+  - symmetry.
+     eapply disj_incl; eauto with cset.
+  - eapply injective_nodup_map; eauto.
+    rewrite of_list_elements. eauto using injective_on_incl with cset.
+    eapply elements_3w.
+Qed.
+
+Instance proper_onv (ϱ:var -> option val)
+  : (@Proper (forall _ : var, option val)
+             (@respectful var (option val) (@_eq var (@SOT_as_OT var (@eq nat) nat_OrderedType))
+                          (@eq (option val))) ϱ) | 0.
+Proof.
+  intuition.
+Qed.
+
+Instance proper_onv' (ϱ:var -> option val)
+  : @Proper (forall _ : var, option val)
+            (@respectful var (option val) (@_eq var (@SOT_as_OT var (@eq nat) nat_OrderedType))
+                         (@_eq (option val) (@option_OrderedType val OrderedType_int))) ϱ | 0.
+Proof.
+  intuition.
+Qed.
+
+Lemma load_agree_after_spill_load (slot : var -> var) (V V':var->option val) VD R M Sp L0
+      (Inj : injective_on VD slot)
+      (Agr1 : agree_on eq R V V')
+      (Agr2 : agree_on eq M V (fun x : var => V' (slot x)))
+      (VDincl:Sp ∪ L0 [<=] VD) (SpR:Sp [<=] R) (LSpM:L0 [<=] Sp ∪ M)
+  : agree_on eq L0 V
+             (V' [slot ⊝ elements Sp <-- V' ⊝ elements Sp]
+                 [elements L0 <-- V' [slot ⊝ elements Sp <-- V' ⊝ elements Sp]
+                           ⊝ slot ⊝ elements L0]).
+Proof.
+  eapply agree_on_update_list; try eapply proper_onv; eauto with len.
+  rewrite of_list_elements. eapply agree_on_empty; eauto with cset.
+  rewrite !lookup_list_map. rewrite map_map. rewrite <- !lookup_list_map.
+  eapply lookup_list_agree. rewrite lookup_list_map.
+  rewrite of_list_elements.
+  etransitivity; [| eapply agree_on_eq_oval, agree_on_update_list_map];
+    [ | eauto with len | eapply proper_var | eapply proper_onv'
+      | eapply injective_on_incl; eauto; rewrite <- VDincl, of_list_elements; clear; cset_tac ].
+  rewrite (set_decomp Sp).
+  eapply agree_on_union.
+  ++ rewrite lookup_list_map.
+    etransitivity; [eapply agree_on_incl; [ eapply Agr1| rewrite <- SpR; clear; cset_tac]|].
+    eapply agree_on_update_list; [ eapply proper_onv | eauto with len |
+                                   | rewrite lookup_list_map; reflexivity ].
+    rewrite of_list_elements. eapply agree_on_empty; clear; cset_tac.
+  ++ rewrite lookup_list_map.
+    eapply agree_on_update_list_dead.
+    eapply agree_on_incl; eauto. rewrite LSpM. clear; cset_tac.
+    rewrite of_list_elements. hnf; intros; cset_tac.
+Qed.
+
+Lemma regs_untouched_after_spill_load (slot : var -> var) (V V' V'':var->option val) VD R M K Sp L0
+      (Agr3 : agree_on eq (R ∪ map slot M ∪ map slot Sp ∪ L0)
+                       (V' [slot ⊝ elements Sp <-- V' ⊝ elements Sp]
+                           [elements L0 <-- V' [slot ⊝ elements Sp <-- V' ⊝ elements Sp]
+                                     ⊝ slot ⊝ elements L0]) V'')
+      (Disj : disj VD (map slot VD)) (Incl : R ∪ M [<=] VD)
+      (Agr1 : agree_on eq R V V')
+      (VDincl:Sp ∪ L0 [<=] VD)
+  :  agree_on eq ((R \ K) \ L0) V V''.
+Proof.
+  etransitivity; [eapply agree_on_incl; [eapply Agr1| clear; cset_tac]|].
+  etransitivity; [|eapply agree_on_incl; [eapply Agr3| clear; cset_tac]].
+  eapply agree_on_update_list_dead.
+  eapply agree_on_update_list_dead. reflexivity.
+  rewrite of_list_map, of_list_elements; eauto.
+  symmetry. eapply disj_incl; eauto; only 2: eauto with cset.
+  rewrite <- Incl. clear; cset_tac.
+  rewrite of_list_elements. clear; hnf; intros; cset_tac.
+Qed.
+
+Lemma regs_agree_after_spill_load (slot : var -> var) (V V' V'':var -> option val) VD R M K Sp L0
+      (Agr3 : agree_on eq (R ∪ map slot M ∪ map slot Sp ∪ L0)
+                       (V' [slot ⊝ elements Sp <-- V' ⊝ elements Sp]
+                           [elements L0 <-- V' [slot ⊝ elements Sp <-- V' ⊝ elements Sp]
+                                     ⊝ slot ⊝ elements L0]) V'')
+      (Inj : injective_on VD slot) (Disj : disj VD (map slot VD)) (Incl : R ∪ M [<=] VD)
+      (Agr1 : agree_on eq R V V')
+      (Agr2 : agree_on eq M V (fun x : var => V' (slot x)))
+      (VDincl:Sp ∪ L0 [<=] VD) (SpR:Sp [<=] R) (LSpM:L0 [<=] Sp ∪ M)
+  : agree_on eq (R \ K ∪ L0) V V''.
+Proof.
+  etransitivity; [|eapply agree_on_incl; [eapply Agr3| clear; cset_tac]].
+  rewrite union_comm, union_exclusive.
+  eapply agree_on_union.
+  -- eapply load_agree_after_spill_load; eauto.
+  -- eapply regs_untouched_after_spill_load; eauto.
+     reflexivity.
+Qed.
+
+Lemma spills_agree_after_spill_load (slot : var -> var) (V V' V'':var->option val) VD R M Sp L0
+      (Inj : injective_on VD slot) (Disj : disj VD (map slot VD)) (Incl : R ∪ M [<=] VD)
+      (Agr1 : agree_on eq R V V')
+      (Agr2 : agree_on eq M V (fun x : var => V' (slot x)))
+      (VDincl:Sp ∪ L0 [<=] VD) (SpR:Sp [<=] R) (LSpM:L0 [<=] Sp ∪ M)
+      (Agr3 : agree_on eq (R ∪ map slot M ∪ map slot Sp ∪ L0)
+                       (V' [slot ⊝ elements Sp <-- V' ⊝ elements Sp]
+                           [elements L0 <-- V' [slot ⊝ elements Sp <-- V' ⊝ elements Sp]
+                                     ⊝ slot ⊝ elements L0]) V'')
+  : agree_on eq Sp V (fun x : var => V'' (slot x)).
+Proof.
+  eapply agree_on_comp; eauto; [ symmetry; eapply agree_on_incl; eauto; clear_all; cset_tac | ].
+  etransitivity; [eapply agree_on_incl; [eapply Agr1| eauto with cset]|].
+  eapply agree_on_update_list_dead_slot; eauto.
+  etransitivity; [| eapply agree_on_eq_oval, agree_on_update_list_map];
+    [ | eauto with len | eapply proper_var | eapply proper_onv'
+      | eapply injective_on_incl; eauto; rewrite <- VDincl, of_list_elements;
+        clear; cset_tac ].
+  eapply agree_on_update_list; [ eapply proper_onv | eauto with len |
+                                 | rewrite lookup_list_map; reflexivity ].
+  eapply agree_on_empty. rewrite of_list_elements. cset_tac.
+  eapply disj_incl; eauto with cset.
+  rewrite of_list_elements, <- Incl, LSpM, <- SpR; reflexivity.
+Qed.
+
+Lemma mem_untouched_after_spill_load (slot : var -> var) (V V' V'':var->option val) VD R M Sp L0
+      (Inj : injective_on VD slot) (Disj : disj VD (map slot VD)) (Incl : R ∪ M [<=] VD)
+      (Agr1 : agree_on eq R V V')
+      (Agr2 : agree_on eq M V (fun x : var => V' (slot x)))
+      (VDincl:Sp ∪ L0 [<=] VD) (SpR:Sp [<=] R) (LSpM:L0 [<=] Sp ∪ M)
+      (Agr3 : agree_on eq (R ∪ map slot M ∪ map slot Sp ∪ L0)
+                       (V' [slot ⊝ elements Sp <-- V' ⊝ elements Sp]
+                           [elements L0 <-- V' [slot ⊝ elements Sp <-- V' ⊝ elements Sp]
+                                     ⊝ slot ⊝ elements L0]) V'')
+  : agree_on eq (M \ Sp) V (fun x : var => V'' (slot x)).
+Proof.
+  etransitivity; [eapply agree_on_incl; [eapply Agr2| eauto with cset ]|].
+  eapply agree_on_comp_both; eauto using proper_onv.
+  etransitivity; [| eapply agree_on_incl; [eapply Agr3| eauto]].
+  - eapply agree_on_update_list_dead.
+    eapply agree_on_update_list_dead. reflexivity.
+    rewrite of_list_map, of_list_elements; eauto.
+    intros.
+    eapply injective_disj; eauto.
+    hnf; intros; cset_tac.
+    eapply injective_on_incl; eauto. rewrite <- Incl. rewrite SpR at 1.
+    cset_tac.
+    rewrite of_list_elements.
+    eapply disj_incl; eauto.
+    rewrite <- Incl, LSpM, <- SpR. eauto. eauto with cset.
+  - rewrite minus_incl. clear. cset_tac.
+Qed.
+
+Lemma mem_agrees_after_spill_load (slot : var -> var) (V V' V'':var->option val) VD R M Sp L0
+      (Agr3 : agree_on eq (R ∪ map slot M ∪ map slot Sp ∪ L0)
+                       (V' [slot ⊝ elements Sp <-- V' ⊝ elements Sp]
+                           [elements L0 <-- V' [slot ⊝ elements Sp <-- V' ⊝ elements Sp]
+                                     ⊝ slot ⊝ elements L0]) V'')
+      (Inj : injective_on VD slot) (Disj : disj VD (map slot VD)) (Incl : R ∪ M [<=] VD)
+      (Agr1 : agree_on eq R V V')
+      (Agr2 : agree_on eq M V (fun x : var => V' (slot x)))
+      (VDincl:Sp ∪ L0 [<=] VD) (SpR:Sp [<=] R) (LSpM:L0 [<=] Sp ∪ M)
+  : agree_on eq (Sp ∪ M) V (fun x : var => V'' (slot x)).
+Proof.
+  rewrite union_exclusive.
+  eapply agree_on_union.
+  -- eapply spills_agree_after_spill_load; try eapply Agr3; eauto.
+  -- eapply mem_untouched_after_spill_load; try eapply Agr3; eauto.
+Qed.
+
+
+Lemma mem_agrees_after_spill_load_update (slot : var -> var) (V V' V'':var->option val) VD R M Sp L0 x v
+      (Agr5 : agree_on eq (Sp ∪ M) V (fun x : var => V'' (slot x)))
+      (Disj : disj VD (map slot VD)) (Incl : R ∪ M [<=] VD) (NotIn: x ∉ Sp ∪ M)
+      (xIn:x ∈ VD)
+      (Agr1 : agree_on eq R V V')
+      (Agr2 : agree_on eq M V (fun x : var => V' (slot x)))
+      (VDincl:Sp ∪ L0 [<=] VD) (SpR:Sp [<=] R) (LSpM:L0 [<=] Sp ∪ M)
+      (Agr3 : agree_on eq (R ∪ map slot M ∪ map slot Sp ∪ L0)
+                       (V' [slot ⊝ elements Sp <-- V' ⊝ elements Sp]
+                           [elements L0 <-- V' [slot ⊝ elements Sp <-- V' ⊝ elements Sp]
+                                     ⊝ slot ⊝ elements L0]) V'')
+  : agree_on eq (Sp ∪ M) (V [x <- ⎣ v ⎦]) (fun x0 : var => (V'' [x <- ⎣ v ⎦]) (slot x0)).
+Proof.
+  eapply agree_on_update_dead_both_comp_right; eauto.
+  eapply disj_incl; eauto. rewrite SpR, Incl. revert xIn; clear. cset_tac.
+  rewrite SpR, Incl. cset_tac.
+Qed.
+
+Lemma RKL_incl X `{OrderedType X} (R K L D D':set X)
+  :  R \ K ∪ L ⊆ R ∪ D ∪ D' ∪ L.
+Proof.
+  cset_tac.
+Qed.
+
+Hint Resolve RKL_incl | 0: cset.
+
+Lemma defined_on_after_spill_load (slot : var -> var) (V V' V'':var->option val) VD R M Sp L0  K
+      (Agr5 : agree_on eq (Sp ∪ M) V (fun x : var => V'' (slot x)))
+      (Disj : disj VD (map slot VD)) (Incl : R ∪ M [<=] VD)
+      (Agr1 : agree_on eq R V V') (Def : defined_on (R ∪ map slot M) V')
+      (Agr2 : agree_on eq M V (fun x : var => V' (slot x)))
+      (VDincl:Sp ∪ L0 [<=] VD) (SpR:Sp [<=] R) (LSpM:L0 [<=] Sp ∪ M)
+      (Agr3 : agree_on eq (R ∪ map slot M ∪ map slot Sp ∪ L0)
+                       (V' [slot ⊝ elements Sp <-- V' ⊝ elements Sp]
+                           [elements L0 <-- V' [slot ⊝ elements Sp <-- V' ⊝ elements Sp]
+                                     ⊝ slot ⊝ elements L0]) V'')
+  : defined_on (R \ K ∪ L0 ∪ map slot (Sp ∪ M)) V''.
+Proof.
+  assert (defined_on Sp V') as DefSp by eauto using defined_on_incl with cset.
+  rewrite union_exclusive.
+  eapply defined_on_union.
+  -- eapply defined_on_agree_eq; [|eapply agree_on_incl;[eapply Agr3|eauto with cset]].
+     rewrite union_comm, union_exclusive. eapply defined_on_union.
+     ++ eapply defined_on_update_list'; eauto with len.
+       rewrite of_list_elements. clear; hnf; intros; cset_tac.
+       eapply defined_on_defined. clear; intuition.
+       rewrite of_list_map, of_list_elements; eauto.
+       eapply defined_on_update_list'; eauto with len.
+       rewrite of_list_map, of_list_elements; eauto.
+       rewrite LSpM. eapply (defined_on_incl Def); eauto.
+       rewrite map_union; eauto. clear; cset_tac.
+       eapply defined_on_defined. clear; intuition. eauto.
+       rewrite of_list_elements. eauto.
+     ++ eapply defined_on_agree_eq; [| eapply agree_on_update_list_dead; try reflexivity].
+       eapply defined_on_update_list'; eauto with len.
+       rewrite of_list_map, of_list_elements; eauto.
+       eapply (defined_on_incl Def). clear; cset_tac.
+       eapply defined_on_defined. clear; intuition. eauto.
+       rewrite of_list_elements. eauto.
+       rewrite of_list_elements. eauto. clear; hnf; intros; cset_tac.
+  -- rewrite map_union; eauto.
+     eapply defined_on_agree_eq; [ | eapply agree_on_incl; [ eapply Agr3| clear; cset_tac]];
+       eauto.
+     eapply defined_on_agree_eq; [| eapply agree_on_update_list_dead; try reflexivity].
+     eapply defined_on_update_list'; eauto with len.
+     rewrite of_list_map, of_list_elements; eauto.
+     eapply (defined_on_incl Def). clear; cset_tac.
+     eapply defined_on_defined. clear; intuition. eauto.
+     rewrite of_list_elements. eauto.
+     rewrite of_list_elements. clear; hnf; intros; cset_tac.
+Qed.
